concurrency/disciplined/CapacityAllocator.i.dfy
@@ -1,0 +1,174 @@
+include "ConcurrencyTools.s.dfy"
+include "../../lib/Checksums/Nonlinear.i.dfy"
+include "ShardedHashTable.i.dfy"
+//include "VerificationObligation.s.dfy"
+
+// we need to import this open to destructure AllocatorBin: dafny doesn't support qualified names in this context
+module CapacityAllocatorTypes {
+  import opened NativeTypes
+  import opened ShardedHashTable
+
+  linear datatype AllocatorBin = AllocatorBin(
+    count: uint32,
+    // NB there's a modularity problem here. Maybe we need to pull the capacity concept
+    // out of the ShardedHashTable so we can refer to it here?
+    glinear resource: ShardedHashTable.Variables)
+}
+
+// separate module to avoid name collision
+module CapacityAllocator {
+  import opened Options
+  import opened NativeTypes
+  import opened ShardedHashTable
+  import opened KeyValueType
+  import opened Mutexes
+  import opened NonlinearLemmas
+  import ARS = ShardedHashTable
+  import opened CapacityAllocatorTypes
+
+  type AllocatorMutex = Mutex<AllocatorBin>
+  type AllocatorMutexTable = seq<AllocatorMutex>
+
+  function BinInv(bin: AllocatorBin): bool
+  {
+    && Valid(bin.resource)
+    && bin.resource == Variables(unitTable(), bin.count as nat, multiset{}, multiset{})
+  }
+
+  function BinCount(): (c: nat)
+    ensures c > 0
+
+  function method BinCountImpl(): (c: uint32)
+    ensures c as nat == BinCount()
+
+  predicate Inv(o: AllocatorMutexTable)
+  {
+    && |o| == BinCount()
+    && (forall i | 0 <= i < BinCount() :: o[i].inv == BinInv)
+  }
+
+  datatype Splitted = Splitted(v': ShardedHashTable.Variables, vi: ShardedHashTable.Variables)
+
+  function Split(v: ShardedHashTable.Variables, amount:nat) : Splitted
+    requires v.Variables?;
+    requires v.table == unitTable()
+    requires v.insert_capacity >= amount
+    requires v.tickets == multiset{}
+    requires v.stubs == multiset{}
+  {
+    var v' := Variables(v.table, v.insert_capacity - amount, multiset{}, multiset{});
+    var vi := Variables(v.table, amount, multiset{}, multiset{});
+    Splitted(v', vi)
+  }
+
+  function method CapacityImpl(): (s: uint32)
+    ensures s as nat == Capacity()
+    
+  predicate CapPreInit(s: ShardedHashTable.Variables)
+  {
+    && s.Variables?
+    && s.table == unitTable()
+    && s.insert_capacity == Capacity()
+    && s.tickets == multiset{}
+    && s.stubs == multiset{}
+  }
+
+  method {:noNLarith} init(glinear in_r: ARS.Variables)
+  returns (mt: AllocatorMutexTable, glinear out_r: ARS.Variables)
+  requires CapPreInit(in_r)
+  ensures Inv(mt)
+  ensures out_r == unit()
+  {
+    glinear var remaining_r := in_r;
+
+    var total_amount :uint32 := CapacityImpl();
+    var bin_count := BinCountImpl();
+    mt := [];
+
+
+    div_leq_numerator(total_amount as int, bin_count as int);
+    var quotient :uint32 := total_amount / bin_count;
+    var reaminder :uint32 := total_amount % bin_count;
+    div_plus_mod_bound(total_amount as nat, bin_count as nat);
+
+    var allocated_sum: nat := 0;
+    var i: uint32 := 0;
+
+    while i < bin_count
+      invariant i == 0 ==> allocated_sum == 0;
+      invariant i > 0 ==> (allocated_sum == quotient as nat * i as nat + reaminder as nat);
+
+      invariant i as int == |mt| <= BinCount()
+      invariant forall j:nat | j < i as int :: mt[j].inv == BinInv
+      invariant remaining_r.Variables?
+      invariant remaining_r.insert_capacity == total_amount as nat - allocated_sum
+      invariant remaining_r.table == unitTable()
+      invariant remaining_r.tickets == multiset{}
+      invariant remaining_r.stubs == multiset{}
+    {
+      if i > 0 {
+        calc >= {
+          remaining_r.insert_capacity - quotient as int;
+          total_amount as int - allocated_sum - quotient as int;
+          total_amount as int - quotient as int * i as int - reaminder as int - quotient as int;
+          {
+            assert i <= bin_count - 1;
+            mul_le_right(quotient as int, i as int, bin_count as int - 1);
+          }
+          total_amount as nat - quotient as nat * (bin_count - 1) as nat - reaminder as nat - quotient as int;
+          {
+            distributive_left(quotient as int, bin_count as int - 1, 1);
+          }
+          total_amount as nat - quotient as nat * bin_count as nat - reaminder as nat;
+          {
+            div_mul_plus_mod(total_amount as int, bin_count as int);
+          }
+          0;
+        }
+
+        assert remaining_r.insert_capacity >= quotient as nat;
+      }
+
+      ghost var prev_sum := allocated_sum;
+      var amount := if i == 0 then quotient + reaminder else quotient;
+      allocated_sum := allocated_sum + amount as nat;
+
+      ghost var splitted := Split(remaining_r, amount as nat);
+      glinear var vi;
+      remaining_r, vi := ARS.split(remaining_r, splitted.v', splitted.vi);
+      assert BinInv(AllocatorBin(amount, vi));
+      var m := new_mutex(AllocatorBin(amount, vi), BinInv);
+      mt := mt + [m];
+
+      i := i + 1;
+
+      assert i > 0;
+
+      if i > 1 {
+        calc == {
+          allocated_sum;
+          prev_sum + quotient as nat;
+          quotient as nat * (i - 1) as nat + reaminder as nat + quotient as nat;
+          {
+            assert quotient as nat * (i - 1) as nat + quotient as nat == i as nat * quotient as nat by {
+              distributive_right(i as int - 1, 1, quotient as int);
+            }
+          }
+          quotient as nat * i as nat + reaminder as nat;
+        }
+      }
+    } 
+
+    calc == {
+      allocated_sum;
+      quotient as nat * bin_count as nat + reaminder as nat;
+      {
+        div_mul_plus_mod(total_amount as int, bin_count as int);
+      }
+      total_amount as nat;
+    }
+
+    out_r := remaining_r;
+  }
+}
+
