concurrency/disciplined/Impl.i.dfy
@@ -1,0 +1,599 @@
+include "CapacityAllocator.i.dfy"
+include "ConcurrencyTools.s.dfy"
+include "ShardedHashTable.i.dfy"
+include "VerificationObligation.s.dfy"
+
+module Impl refines VerificationObligation {
+  import opened Options
+  import opened HTResource
+  import opened KeyValueType
+  import opened Mutexes
+  import opened CapacityAllocatorTypes
+  import CAP = CapacityAllocator
+
+  linear datatype Row = Row(
+    entry: HTResource.Entry,
+    glinear resource: HTResource.R)
+
+  type RowMutex = Mutex<Row>
+  type RowMutexTable = seq<RowMutex>
+
+  datatype Variables = Variables(row_mutexes: RowMutexTable, allocator: CAP.AllocatorMutexTable)
+
+  function RowInv(index: nat, row: Row): bool
+  {
+    && Valid(row.resource)
+    && 0 <= index as nat < FixedSize()
+    && row.resource == oneRowResource(index as nat, Info(row.entry, Free), 0)
+  }
+
+  predicate Inv(v: Variables) {
+    && CAP.Inv(v.allocator)
+    && |v.row_mutexes| == HTResource.FixedSize()
+    && (forall i | 0 <= i < FixedSize()
+      :: v.row_mutexes[i].inv == ((row) => RowInv(i, row)))
+  }
+
+  datatype Splitted = Splitted(r':ARS.R, ri:ARS.R)
+
+  function Split(r:ARS.R, i:nat) : Splitted
+    requires r.R?;
+    requires r.tickets == multiset{}
+    requires r.stubs == multiset{}
+  {
+    var r' := R(seq(|r.table|, (j) requires 0<=j<|r.table| => if j!=i then r.table[j] else None), r.insert_capacity, multiset{}, multiset{});
+    var ri := R(seq(|r.table|, (j) requires 0<=j<|r.table| => if j==i then r.table[j] else None), 0, multiset{}, multiset{});
+    Splitted(r', ri)
+  }
+
+  method init(glinear in_r: ARS.R)
+  returns (v: Variables, glinear out_r: ARS.R)
+  // requires ARS.Init(i)
+  ensures Inv(v)
+  ensures out_r == unit()
+  {
+    glinear var remaining_r := in_r;
+    var row_mutexes : RowMutexTable:= [];
+    var i:uint32 := 0;
+    while i < FixedSizeImpl()
+      invariant i as int == |row_mutexes| <= FixedSize()
+      invariant forall j:nat | j<i as int :: && row_mutexes[j].inv == (row) => RowInv(j, row)
+      invariant remaining_r.R?
+      invariant remaining_r.tickets == multiset{}
+      invariant remaining_r.stubs == multiset{} 
+      invariant forall k:nat | k < i as int :: remaining_r.table[k].None?
+      invariant forall l:nat | i as int <= l < |remaining_r.table| :: remaining_r.table[l] == Some(Info(Empty, Free))
+      invariant remaining_r.insert_capacity == Capacity()
+    {
+      ghost var splitted := Split(remaining_r, i as int);
+      glinear var ri;
+      remaining_r, ri := ARS.split(remaining_r, splitted.r', splitted.ri);
+      var m := new_mutex<Row>(Row(Empty, ri), (row) => RowInv(i as nat, row));
+      row_mutexes := row_mutexes + [m];
+      i := i + 1;
+    }
+
+    var allocator: CAP.AllocatorMutexTable;
+    allocator, out_r := CAP.init(remaining_r);
+
+    v := Variables(row_mutexes, allocator);
+
+    assert forall i:nat | i < FixedSize() :: out_r.table[i].None?;
+    assert out_r == unit();
+  }
+
+  predicate method shouldHashGoBefore(search_h: uint32, slot_h: uint32, slot_idx: uint32) 
+    ensures shouldHashGoBefore(search_h, slot_h, slot_idx) == ShouldHashGoBefore(search_h as int, slot_h as int, slot_idx as int)
+  {
+    || search_h < slot_h <= slot_idx // normal case
+    || slot_h <= slot_idx < search_h // search_h wraps around the end of array
+    || slot_idx < search_h < slot_h// search_h, slot_h wrap around the end of array
+  }
+
+  function method getNextIndex(slot_idx: uint32) : uint32
+    requires slot_idx < FixedSizeImpl()
+  {
+    if slot_idx == FixedSizeImpl() - 1 then 0 else slot_idx + 1
+  }
+
+  function DistanceToSlot(src: uint32, dst: uint32) : nat
+    requires src < FixedSizeImpl()
+    requires dst < FixedSizeImpl()
+  {
+    if src >= dst
+      then (dst as int - src as int + FixedSize() as int)
+      else (dst as int - src as int)
+  }
+
+  method doQuery(v: Variables, input: Ifc.Input, rid: int, glinear in_r: ARS.R)
+  returns (output: Ifc.Output, glinear out_r: ARS.R)
+    decreases *
+    requires Inv(v)
+    requires input.QueryInput?
+    requires isInputResource(in_r, rid, input)
+    ensures out_r == ARS.output_stub(rid, output)
+  {
+    var query_ticket := Ticket(rid, input);
+    var key := input.key;
+    var hash_idx := hash(key);
+    var slot_idx := hash_idx;
+
+    linear var row; glinear var handle;
+    row, handle := v.row_mutexes[slot_idx].acquire();
+    linear var Row(entry, row_r) := row;
+    glinear var r := ARS.join(in_r, row_r);
+
+    ghost var r' := oneRowResource(hash_idx as nat, Info(entry, Querying(rid, key)), 0);
+    assert ProcessQueryTicket(r, r', query_ticket);
+
+    var step := ProcessQueryTicketStep(query_ticket);
+    r := easy_transform_step(r, r', step);
+
+    while true 
+      invariant Inv(v);
+      invariant 0 <= slot_idx < FixedSizeImpl();
+      invariant r == oneRowResource(slot_idx as nat, Info(entry, Querying(rid, key)), 0);
+      invariant handle.m == v.row_mutexes[slot_idx];
+      decreases *
+    {
+      var slot_idx' := getNextIndex(slot_idx);
+
+      match entry {
+        case Empty => {
+          output := MapIfc.QueryOutput(NotFound);
+          step := QueryNotFoundStep(slot_idx as nat);
+        }
+        case Full(KV(entry_key, value)) => {
+          if entry_key == key {
+            step := QueryDoneStep(slot_idx as nat);
+            output := MapIfc.QueryOutput(Found(value));
+          } else {
+            var should_go_before := shouldHashGoBefore(hash_idx, hash(entry_key), slot_idx);
+
+            if !should_go_before {
+              step := QuerySkipStep(slot_idx as nat);
+            } else {
+              output := MapIfc.QueryOutput(NotFound);
+              step := QueryNotFoundStep(slot_idx as nat);
+            }
+          }
+        }
+      }
+
+      if !step.QuerySkipStep? {
+        // this test is required for termination, but is not enforced by verification
+        // because we are using decreases *
+        break;
+      }
+
+      // if slot_idx' == hash_idx {
+      //   QueryUnreachableState(r, slot_idx as nat);
+      //   break;
+      // }
+
+      linear var next_row; glinear var next_handle;
+      next_row, next_handle := v.row_mutexes[slot_idx'].acquire();
+      linear var Row(next_entry, next_row_r) := next_row;
+      r := ARS.join(r, next_row_r);
+
+      r' := twoRowsResource(slot_idx as nat, Info(entry, Free), slot_idx' as nat, Info(next_entry, Querying(rid, key)), 0);
+      r := easy_transform_step(r, r', step);
+
+      glinear var rmutex;
+      ghost var left := oneRowResource(slot_idx' as nat, Info(next_entry, Querying(rid, key)), 0);
+      ghost var right := oneRowResource(slot_idx as nat, Info(entry, Free), 0);
+      r, rmutex := ARS.split(r, left, right);
+      v.row_mutexes[slot_idx].release(Row(entry, rmutex), handle);
+
+      slot_idx := slot_idx';
+      entry := next_entry;
+      handle := next_handle;
+    }
+    
+    // assert step.QueryNotFoundStep? || step.QueryDoneStep?;
+    r' := R(oneRowTable(slot_idx as nat, Info(entry, Free)), 0, multiset{}, multiset{Stub(rid, output)}); 
+    r := easy_transform_step(r, r', step);
+
+    glinear var rmutex;
+    r, rmutex := ARS.split(r, 
+      ARS.output_stub(rid, output), 
+      oneRowResource(slot_idx as nat, Info(entry, Free), 0));
+    v.row_mutexes[slot_idx].release(Row(entry, rmutex), handle);
+
+    out_r := r;
+  }
+
+  method acquireCapacity(v: Variables, thread_id: uint32)
+  returns (linear cap: AllocatorBin, glinear cap_handle: MutexHandle<AllocatorBin>, tid: uint32)
+    decreases *
+    requires Inv(v)
+    ensures cap.resource == unit().(insert_capacity := cap.count as nat)
+    ensures 0 < cap.count
+    ensures tid < CAP.BinCountImpl()
+    ensures cap_handle.m == v.allocator[tid]
+  {
+    // thread_id is a hint for the bin we're supposed to use. 
+    // tid is the actual place we found the capacity (in case we had to steal it from someone else) 
+    tid := if thread_id >= CAP.BinCountImpl() then 0 else thread_id;
+    cap, cap_handle := v.allocator[tid].acquire();
+
+    while true
+      invariant tid < CAP.BinCountImpl()
+      invariant cap.resource == unit().(insert_capacity := cap.count as nat)
+      invariant cap_handle.m == v.allocator[tid]
+      decreases *
+    {
+      if 0 < cap.count {
+        break;
+      }
+
+      v.allocator[tid].release(cap, cap_handle);
+
+      tid := tid + 1;
+      tid := if tid >= CAP.BinCountImpl() then 0 else tid;
+
+      cap, cap_handle := v.allocator[tid].acquire();
+    }
+  }
+
+  method doInsert(v: Variables, input: Ifc.Input, rid: int, thread_id: uint32, glinear in_r: ARS.R)
+  returns (output: Ifc.Output, glinear out_r: ARS.R)
+    requires Inv(v)
+    requires input.InsertInput?
+    requires isInputResource(in_r, rid, input)
+    ensures out_r == ARS.output_stub(rid, output)
+    decreases *
+  {
+    var allocator := v.allocator;
+
+    var query_ticket := Ticket(rid, input);
+    var key, inital_key := input.key, input.key;
+    var kv := KV(key, input.value);
+    output := MapIfc.InsertOutput(true);
+
+    var hash_idx := hash(key);
+    var initial_hash_idx := hash_idx;
+    var slot_idx := hash_idx;
+
+    linear var cap; glinear var cap_handle; var tid;
+    cap, cap_handle, tid := acquireCapacity(v, thread_id);
+    linear var AllocatorBin(count, cap_r) := cap;
+    glinear var r := ARS.join(in_r, cap_r);
+
+    linear var row; glinear var handle;
+    row, handle := v.row_mutexes[slot_idx].acquire();
+    linear var Row(entry, row_r) := row;
+    r := ARS.join(r, row_r);
+
+    count := count - 1;
+
+    var step := ProcessInsertTicketStep(query_ticket);
+    ghost var r' := oneRowResource(hash_idx as nat, Info(entry, Inserting(rid, kv, inital_key)), count as nat);
+    r := easy_transform_step(r, r', step);
+    glinear var rmutex;
+
+    while true 
+      invariant Inv(v);
+      invariant 0 <= slot_idx < FixedSizeImpl()
+      invariant r == oneRowResource(slot_idx as nat, Info(entry, Inserting(rid, kv, inital_key)), count as nat)
+      invariant kv.key == key
+      invariant hash_idx == hash(key)
+      invariant handle.m == v.row_mutexes[slot_idx];
+      decreases *
+    {
+      var slot_idx' := getNextIndex(slot_idx);
+      var new_kv;
+
+      match entry {
+        case Empty => {
+          step := InsertDoneStep(slot_idx as nat);
+        }
+        case Full(KV(entry_key, value)) => {
+          new_kv := KV(entry_key, value);
+          if entry_key == key {
+            step := InsertUpdateStep(slot_idx as nat);
+          } else {
+            var should_go_before := shouldHashGoBefore(hash_idx, hash(entry_key), slot_idx);
+            if !should_go_before {
+              step := InsertSkipStep(slot_idx as nat);
+            } else {
+              step := InsertSwapStep(slot_idx as nat);
+            }
+          }
+        }
+      }
+
+      if step.InsertDoneStep? || step.InsertUpdateStep? {
+        break;
+      }
+
+      linear var next_row; glinear var next_handle;
+      next_row, next_handle := v.row_mutexes[slot_idx'].acquire();
+      linear var Row(next_entry, next_row_r) := next_row;
+      r := ARS.join(r, next_row_r);
+
+      if step.InsertSwapStep? {
+        entry := Full(kv);
+        kv := new_kv;
+        key := new_kv.key;
+      }
+  
+      r' := twoRowsResource(slot_idx as nat, Info(entry, Free), slot_idx' as nat, Info(next_entry, Inserting(rid, kv, inital_key)), count as nat);
+      r := easy_transform_step(r, r', step);
+
+      ghost var left := oneRowResource(slot_idx' as nat, Info(next_entry, Inserting(rid, kv, inital_key)), count as nat);
+      ghost var right := oneRowResource(slot_idx as nat, Info(entry, Free), 0);
+
+      r, rmutex := ARS.split(r, left, right);
+      v.row_mutexes[slot_idx].release(Row(entry, rmutex), handle);
+
+      slot_idx := slot_idx';
+      entry := next_entry;
+      hash_idx := hash(key);
+      handle := next_handle;
+    }
+
+    // assert step.InsertDoneStep? || step.InsertUpdateStep?;
+    count := if step.InsertDoneStep? then count else count + 1;
+    r' := R(oneRowTable(slot_idx as nat, Info(Full(kv), Free)), count as nat, multiset{}, multiset{Stub(rid, output)});
+    r := easy_transform_step(r, r', step);
+
+    r, rmutex := ARS.split(r, 
+      ARS.output_stub(rid, output).(insert_capacity := count as nat), 
+      oneRowResource(slot_idx as nat, Info(Full(kv), Free), 0));
+    v.row_mutexes[slot_idx].release(Row(Full(kv), rmutex), handle);
+
+    glinear var rcap;
+    r, rcap := ARS.split(r,
+      ARS.output_stub(rid, output), 
+      unit().(insert_capacity := count as nat));
+
+    allocator[tid].release(AllocatorBin(count, rcap), cap_handle);
+
+    out_r := r;
+  }
+
+  method doRemoveFound(v: Variables, rid: int, 
+    slot_idx: uint32,
+    hash_idx: uint32,
+    inital_key: Key,
+    entry: Entry,
+    thread_id: uint32,
+    glinear handle: MutexHandle<Row>,
+    glinear r: ARS.R)
+  
+    returns (output: Ifc.Output, glinear out_r: ARS.R)
+    decreases *
+    requires Inv(v)
+    requires 0 <= slot_idx < FixedSizeImpl()
+    requires 0 <= hash_idx < FixedSizeImpl()
+    requires r == oneRowResource(slot_idx as nat, Info(entry, Removing(rid, inital_key)), 0);
+    requires entry.Full? && entry.kv.key == inital_key
+    requires hash(inital_key) == hash_idx
+    requires handle.m == v.row_mutexes[slot_idx]
+    ensures out_r == ARS.output_stub(rid, output)
+  {
+    var found_value := entry.kv.val;
+    // var allocator := v.allocator;
+
+    var slot_idx := slot_idx;
+    var slot_idx' := getNextIndex(slot_idx);
+
+    glinear var handle := handle;
+    glinear var rmutex;
+
+    linear var next_row; glinear var next_handle;
+    next_row, next_handle := v.row_mutexes[slot_idx'].acquire();
+    linear var Row(next_entry, next_row_r) := next_row;
+    glinear var r := ARS.join(r, next_row_r);
+
+    var step := RemoveFoundItStep(slot_idx as nat);
+    var r' := twoRowsResource(
+        slot_idx as nat, Info(Empty, RemoveTidying(rid, inital_key, found_value)),
+        slot_idx' as nat, Info(next_entry, Free),
+        0);
+    r := easy_transform_step(r, r', step);
+
+    while true
+      invariant Inv(v);
+      invariant 0 <= slot_idx < FixedSizeImpl()
+      invariant r == twoRowsResource(
+        slot_idx as nat, Info(Empty, RemoveTidying(rid, inital_key, found_value)),
+        NextPos(slot_idx as nat), Info(next_entry, Free),
+        0)
+      invariant handle.m == v.row_mutexes[slot_idx]
+      invariant next_handle.m == v.row_mutexes[NextPos(slot_idx as nat)]
+      decreases *
+    {
+      slot_idx' := getNextIndex(slot_idx);
+
+      if next_entry.Empty? || (next_entry.Full? && hash(next_entry.kv.key) == slot_idx') {
+        assert DoneTidying(r, slot_idx as nat);
+        break;
+      }
+
+      ghost var r' := twoRowsResource(
+        slot_idx as nat, Info(next_entry, Free),
+        slot_idx' as nat, Info(Empty, RemoveTidying(rid, inital_key, found_value)),
+        0);
+      r := easy_transform_step(r, r', RemoveTidyStep(slot_idx as nat));
+
+      ghost var left := oneRowResource(slot_idx' as nat, Info(Empty, RemoveTidying(rid, inital_key, found_value)), 0);
+      ghost var right := oneRowResource(slot_idx as nat, Info(next_entry, Free), 0);
+
+      r, rmutex := ARS.split(r, left, right);
+      v.row_mutexes[slot_idx].release(Row(next_entry, rmutex), handle);
+
+      slot_idx := slot_idx';
+      slot_idx' := getNextIndex(slot_idx);
+      handle := next_handle;
+
+      next_row, next_handle := v.row_mutexes[slot_idx'].acquire();
+      linear var Row(next_entry', next_row_r) := next_row;
+      next_entry := next_entry';
+      r := ARS.join(r, next_row_r);
+    }
+
+    assert DoneTidying(r, slot_idx as nat);
+
+    slot_idx' := getNextIndex(slot_idx);
+    output := MapIfc.RemoveOutput(true);
+
+    linear var cap; glinear var cap_handle; var tid;
+    cap, cap_handle, tid := acquireCapacity(v, thread_id);
+    linear var AllocatorBin(count, cap_r) := cap;
+    r := ARS.join(r, cap_r);
+
+    r' := R(
+      twoRowsTable(slot_idx as nat, Info(Empty, Free), slot_idx' as nat, Info(next_entry, Free)),
+      count as nat + 1,
+      multiset{},
+      multiset{ Stub(rid, output) }
+    );
+
+    step := RemoveDoneStep(slot_idx as nat);
+    r := easy_transform_step(r, r', step);
+
+    ghost var left := R(
+      oneRowTable(slot_idx' as nat, Info(next_entry, Free)),
+      count as nat + 1,
+      multiset{},
+      multiset{ Stub(rid, output) });
+    ghost var right := oneRowResource(slot_idx as nat, Info(Empty, Free), 0);
+
+    r, rmutex := ARS.split(r, left, right);
+    v.row_mutexes[slot_idx].release(Row(Empty, rmutex), handle);
+
+    r, rmutex := ARS.split(r, 
+      ARS.output_stub(rid, output).(insert_capacity := count as nat + 1), 
+      oneRowResource(slot_idx' as nat, Info(next_entry, Free), 0));
+    v.row_mutexes[slot_idx'].release(Row(next_entry, rmutex), next_handle);
+
+    r, cap_r := ARS.split(r,
+      ARS.output_stub(rid, output), 
+      unit().(insert_capacity := count as nat + 1));
+  
+    v.allocator[tid].release(AllocatorBin(count+1, cap_r), cap_handle);
+
+    out_r := r;
+  }
+
+  method doRemove(v: Variables, input: Ifc.Input, rid: int, thread_id: uint32, glinear in_r: ARS.R)
+    returns (output: Ifc.Output, glinear out_r: ARS.R)
+    decreases *
+
+    requires Inv(v)
+    requires input.RemoveInput?
+    requires isInputResource(in_r, rid, input)
+    ensures out_r == ARS.output_stub(rid, output)
+  {
+    var query_ticket := Ticket(rid, input);
+    var key := input.key;
+    var hash_idx := hash(key); var slot_idx := hash_idx;
+
+    linear var row; glinear var handle;
+    row, handle := v.row_mutexes[slot_idx].acquire();
+
+    linear var Row(entry, row_r) := row;
+    glinear var r := ARS.join(in_r, row_r);
+
+    var slot_idx' :uint32;
+    glinear var rmutex;
+
+    glinear var r' := oneRowResource(hash_idx as nat, Info(entry, Removing(rid, key)), 0);
+    var step : Step := ProcessRemoveTicketStep(query_ticket);
+    r := easy_transform_step(r, r', step);
+
+    while true 
+      invariant Inv(v);
+      invariant 0 <= slot_idx < FixedSizeImpl();
+      invariant r == oneRowResource(slot_idx as nat, Info(entry, Removing(rid, key)), 0)
+      invariant step.RemoveNotFoundStep? ==> 
+        (entry.Full? && shouldHashGoBefore(hash_idx, hash(entry.kv.key), slot_idx))
+      invariant step.RemoveTidyStep? ==> (
+        && TidyEnabled(r, slot_idx as nat)
+        && KnowRowIsFree(r, NextPos(slot_idx as nat)))
+      invariant handle.m == v.row_mutexes[slot_idx]
+      decreases *
+    {
+      var slot_idx' := getNextIndex(slot_idx);
+
+      match entry {
+        case Empty => {
+          step := RemoveNotFoundStep(slot_idx as nat);
+        }
+        case Full(KV(entry_key, value)) => {
+          if entry_key == key {
+            step := RemoveFoundItStep(slot_idx as nat);
+          } else {
+            var should_go_before := shouldHashGoBefore(hash_idx, hash(entry_key), slot_idx);
+
+            if !should_go_before {
+              step := RemoveSkipStep(slot_idx as nat);
+            } else {
+              step := RemoveNotFoundStep(slot_idx as nat);
+            }
+          }
+        }
+      }
+
+      if step.RemoveNotFoundStep? || step.RemoveFoundItStep? {
+        break;
+      }
+
+      linear var next_row; glinear var next_handle;
+      next_row, next_handle := v.row_mutexes[slot_idx'].acquire();
+      linear var Row(next_entry, next_row_r) := next_row;
+      r := ARS.join(r, next_row_r);
+
+      r' := twoRowsResource(slot_idx as nat, Info(entry, Free), slot_idx' as nat, Info(next_entry, Removing(rid, key)), 0);
+      r := easy_transform_step(r, r', step);
+
+      ghost var left := oneRowResource(slot_idx' as nat, Info(next_entry, Removing(rid, key)), 0);
+      ghost var right := oneRowResource(slot_idx as nat, Info(entry, Free), 0);
+      r, rmutex := ARS.split(r, left, right);
+      v.row_mutexes[slot_idx].release(Row(entry, rmutex), handle);
+
+      slot_idx := slot_idx';
+      entry := next_entry;
+      handle := next_handle;
+    }
+
+    if step.RemoveNotFoundStep? {
+      output := MapIfc.RemoveOutput(false);
+      r' := R(oneRowTable(slot_idx as nat, Info(entry, Free)), 0, multiset{}, multiset{Stub(rid, output)}); 
+      r := easy_transform_step(r, r', step);
+      ghost var left := ARS.output_stub(rid, output);
+      ghost var right := oneRowResource(slot_idx as nat, Info(entry, Free), 0);
+      r, rmutex := ARS.split(r, left, right);
+      v.row_mutexes[slot_idx].release(Row(entry, rmutex), handle);
+    } else {
+      output, r := doRemoveFound(v, rid, slot_idx, hash_idx, key, entry, thread_id, handle, r);
+    }
+
+    out_r := r;
+  }
+
+  method call(v: Variables, input: Ifc.Input, rid: int, glinear in_r: ARS.R, thread_id: uint32)
+    returns (output: Ifc.Output, glinear out_r: ARS.R)
+    decreases *
+  // requires Inv(o)
+  // requires ticket == ARS.input_ticket(rid, key)
+    ensures out_r == ARS.output_stub(rid, output)
+  {
+    // Find the ticket.
+    assert |in_r.tickets| == 1;
+    var the_ticket :| the_ticket in in_r.tickets;
+
+    if the_ticket.input.QueryInput? {
+      output, out_r := doQuery(v, input, rid, in_r);
+    } else if the_ticket.input.InsertInput? {
+      output, out_r := doInsert(v, input, rid, thread_id, in_r);
+    } else if the_ticket.input.RemoveInput? {
+      output, out_r := doRemove(v, input, rid, thread_id, in_r);
+    } else {
+      out_r := in_r;
+      assert false;
+    }
+  }
+}
